timesyn/CaseStudies/abp/SenderAutomaton.thy
@@ -1,113 +1,86 @@
+(*
+ * DO NOT MODIFY!
+ * This file was generated from Sender.maa and will be overridden when changed. To change
+ * permanently, consider changing the model itself.
+ *
+ * Generated on Jul 3, 2018 6:22:45 PM by transformer 1.0.0
+ *)
 theory SenderAutomaton
 
-imports "../../../untimed/CaseStudy/Automaton" "../../tsynStream" "../../tsynBundle" 
+imports "../AutomatonPrelude"
 
 begin
-
-fun prepend:: "nat list \<Rightarrow> nat \<Rightarrow> nat list" where
-"prepend xs x= x#xs"
 
 (* This are the actual states from MAA *)
 datatype SenderSubstate = Sf | St
 
 (* And these have also the variables *)
-datatype SenderState = State SenderSubstate "nat list"
+datatype SenderState = State SenderSubstate (* buffer = *) "nat list"
 
 fun getSubState :: "SenderState \<Rightarrow> SenderSubstate" where
-    "getSubState (State state_s automaton_buffer) = state_s"
+"getSubState (State state_s automaton_buffer) = state_s"
 
 fun getBuffer :: "SenderState \<Rightarrow> nat list" where
 "getBuffer (State _ automaton_buffer) = automaton_buffer"
     
 
-datatype Sender = A "nat" | B "bool" | C "(nat\<times>bool)"
-instance Sender :: countable
-apply(intro_classes)
-by(countable_datatype)
 
-abbreviation input_i_c1 :: "channel" ("\<guillemotright>i") where
-"\<guillemotright>i \<equiv> c1"
+fun senderTransitionH :: "(SenderState \<times> (abpMessage tsyn \<times> abpMessage tsyn)) \<Rightarrow> (SenderState \<times> abpMessage tsyn SB)" where
+    "senderTransitionH (State Sf automaton_buffer, ((*i\<mapsto>*)Msg (Nat a), (*as\<mapsto>*)Msg (Bool b))) = 
+       (if((size automaton_buffer)>1 \<and> b=False) then ((State St ((prepend (butlast automaton_buffer))a),(createDsBundle (Pair (last (butlast automaton_buffer)) True ))))
+       else if((size automaton_buffer)=0) then ((State Sf ((prepend automaton_buffer)a),(createDsBundle (Pair a False ))))
+       else if((size automaton_buffer)=1 \<and> b=False) then ((State St ((prepend (butlast automaton_buffer))a),(createDsBundle (Pair a True ))))
+       else if((size automaton_buffer)>0 \<and> b=True) then ((State Sf ((prepend automaton_buffer)a),(createDsBundle (Pair (last automaton_buffer) False ))))
+       else  (State Sf automaton_buffer, ((tsynbNull (\<C> ''ds'')))))"  |
 
-abbreviation input_as_c2 :: "channel" ("\<guillemotright>as") where
-"\<guillemotright>as \<equiv> c2"
+    "senderTransitionH (State Sf automaton_buffer, ((*i\<mapsto>*)Msg (Nat a), (*as\<mapsto>*)null)) = 
+       (if((size automaton_buffer)=0) then ((State Sf ((prepend automaton_buffer)a),(createDsBundle (Pair a False ))))
+       else if((size automaton_buffer)>0) then ((State Sf ((prepend automaton_buffer)a),(createDsBundle (Pair (last automaton_buffer) False ))))
+       else  (State Sf automaton_buffer, ((tsynbNull (\<C> ''ds'')))))"  |
 
-abbreviation output_ds_c3 :: "channel" ("ds\<guillemotright>") where
-"ds\<guillemotright> \<equiv> c3"
+    "senderTransitionH (State Sf automaton_buffer, ((*i\<mapsto>*)null, (*as\<mapsto>*)Msg (Bool b))) = 
+       (if((size automaton_buffer)=0) then ((State Sf automaton_buffer,(tsynbNull (\<C> ''ds''))))
+       else if((size automaton_buffer)=1 \<and> b=False) then ((State St ((butlast automaton_buffer)),(tsynbNull (\<C> ''ds''))))
+       else if((size automaton_buffer)>0 \<and> b=True) then ((State Sf automaton_buffer,(createDsBundle (Pair (last automaton_buffer) False ))))
+       else if((size automaton_buffer)>1 \<and> b=False) then ((State St ((butlast automaton_buffer)),(createDsBundle (Pair (last (butlast automaton_buffer)) True ))))
+       else  (State Sf automaton_buffer, ((tsynbNull (\<C> ''ds'')))))"  |
 
-instantiation Sender :: message
-begin
-fun ctype_Sender :: "channel  \<Rightarrow> Sender set" where
-    "ctype_Sender \<guillemotright>i = range A" | 
-    "ctype_Sender \<guillemotright>as = range B" | 
-    "ctype_Sender ds\<guillemotright> = range C" 
-instance
-by(intro_classes)
-end
+    "senderTransitionH (State Sf automaton_buffer, ((*i\<mapsto>*)null, (*as\<mapsto>*)null)) = 
+       (if((size automaton_buffer)>0) then ((State Sf automaton_buffer,(createDsBundle (Pair (last automaton_buffer) False ))))
+       else if((size automaton_buffer)=0) then ((State Sf automaton_buffer,(tsynbNull (\<C> ''ds''))))
+       else  (State Sf automaton_buffer, ((tsynbNull (\<C> ''ds'')))))"  |
 
-lift_definition createDsOutput :: "(nat\<times>bool) \<Rightarrow> Sender tsyn SB" is
-    "\<lambda>b. [ ds\<guillemotright> \<mapsto> \<up>(Msg (C b))]"
-unfolding ubWell_def
-unfolding usclOkay_stream_def
-unfolding ctype_tsyn_def
-by simp
+    "senderTransitionH (State St automaton_buffer, ((*i\<mapsto>*)Msg (Nat a), (*as\<mapsto>*)Msg (Bool b))) = 
+       (if((size automaton_buffer)>1 \<and> b=True) then ((State Sf ((prepend (butlast automaton_buffer))a),(createDsBundle (Pair (last (butlast automaton_buffer)) False ))))
+       else if((size automaton_buffer)>0 \<and> b=False) then ((State St ((prepend automaton_buffer)a),(createDsBundle (Pair (last automaton_buffer) True ))))
+       else if((size automaton_buffer)=1 \<and> b=True) then ((State Sf ((prepend (butlast automaton_buffer))a),(createDsBundle (Pair a False ))))
+       else if((size automaton_buffer)=0) then ((State St ((prepend automaton_buffer)a),(createDsBundle (Pair a True ))))
+       else  (State St automaton_buffer, ((tsynbNull (\<C> ''ds'')))))"  |
 
+    "senderTransitionH (State St automaton_buffer, ((*i\<mapsto>*)null, (*as\<mapsto>*)Msg (Bool b))) = 
+       (if((size automaton_buffer)>1 \<and> b=True) then ((State Sf ((butlast automaton_buffer)),(createDsBundle (Pair (last (butlast automaton_buffer)) False ))))
+       else if((size automaton_buffer)=0) then ((State St automaton_buffer,(tsynbNull (\<C> ''ds''))))
+       else if((size automaton_buffer)=1 \<and> b=True) then ((State Sf ((butlast automaton_buffer)),(tsynbNull (\<C> ''ds''))))
+       else if((size automaton_buffer)>0 \<and> b=False) then ((State St automaton_buffer,(createDsBundle (Pair (last automaton_buffer) True ))))
+       else  (State St automaton_buffer, ((tsynbNull (\<C> ''ds'')))))"  |
 
-fun senderTransitionH :: "(SenderState \<times> (Sender tsyn \<times> Sender tsyn)) \<Rightarrow> (SenderState \<times> Sender tsyn SB)" where
-    "senderTransitionH (State Sf automaton_buffer, (Msg (A a), Msg (B b))) = 
-       (if((size automaton_buffer)>0 \<and> b=True) then ((State Sf ((prepend automaton_buffer)a),(createDsOutput (Pair (last automaton_buffer) False ))))
-       else if((size automaton_buffer)>1 \<and> b=False) then ((State St ((prepend (butlast automaton_buffer))a),(createDsOutput (Pair (last (butlast automaton_buffer)) True ))))
-       else if((size automaton_buffer)=1 \<and> b=False) then ((State St ((prepend (butlast automaton_buffer))a),(createDsOutput (Pair a True ))))
-       else if((size automaton_buffer)=0) then ((State Sf ((prepend automaton_buffer)a),(createDsOutput (Pair a False ))))
-       else  (State Sf automaton_buffer, ((tsynbNull ds\<guillemotright>))))"  |
+    "senderTransitionH (State St automaton_buffer, ((*i\<mapsto>*)Msg (Nat a), (*as\<mapsto>*)null)) = 
+       (if((size automaton_buffer)>0) then ((State St ((prepend automaton_buffer)a),(createDsBundle (Pair (last automaton_buffer) True ))))
+       else if((size automaton_buffer)=0) then ((State St ((prepend automaton_buffer)a),(createDsBundle (Pair a True ))))
+       else  (State St automaton_buffer, ((tsynbNull (\<C> ''ds'')))))"  |
 
-    "senderTransitionH (State Sf automaton_buffer, (null, Msg (B b))) = 
-       (if((size automaton_buffer)>0 \<and> b=True) then ((State Sf automaton_buffer,(createDsOutput (Pair (last automaton_buffer) False ))))
-       else if((size automaton_buffer)>1 \<and> b=False) then ((State St ((butlast automaton_buffer)),(createDsOutput (Pair (last (butlast automaton_buffer)) True ))))
-       else if((size automaton_buffer)=0) then ((State Sf automaton_buffer,(tsynbNull ds\<guillemotright>)))
-       else if((size automaton_buffer)=1 \<and> b=False) then ((State St ((butlast automaton_buffer)),(tsynbNull ds\<guillemotright>)))
-       else  (State Sf automaton_buffer, ((tsynbNull ds\<guillemotright>))))"  |
+    "senderTransitionH (State St automaton_buffer, ((*i\<mapsto>*)null, (*as\<mapsto>*)null)) = 
+       (if((size automaton_buffer)>0) then ((State St automaton_buffer,(createDsBundle (Pair (last automaton_buffer) True ))))
+       else if((size automaton_buffer)=0) then ((State St automaton_buffer,(tsynbNull (\<C> ''ds''))))
+       else  (State St automaton_buffer, ((tsynbNull (\<C> ''ds'')))))"  
 
-    "senderTransitionH (State Sf automaton_buffer, (Msg (A a), null)) = 
-       (if((size automaton_buffer)=0) then ((State Sf ((prepend automaton_buffer)a),(createDsOutput (Pair a False ))))
-       else if((size automaton_buffer)>0) then ((State Sf ((prepend automaton_buffer)a),(createDsOutput (Pair (last automaton_buffer) False ))))
-       else  (State Sf automaton_buffer, ((tsynbNull ds\<guillemotright>))))"  |
+fun senderTransition :: "(SenderState \<times> (channel \<rightharpoonup> abpMessage tsyn)) \<Rightarrow> (SenderState \<times> abpMessage tsyn SB)" where
+"senderTransition (s,f) = (if dom(f) = {\<C> ''i'',\<C> ''as''} then senderTransitionH (s,(f\<rightharpoonup>\<C> ''i'',f\<rightharpoonup>\<C> ''as'')) else undefined)"
 
-    "senderTransitionH (State Sf automaton_buffer, (null, null)) = 
-       (if((size automaton_buffer)>0) then ((State Sf automaton_buffer,(createDsOutput (Pair (last automaton_buffer) False ))))
-       else if((size automaton_buffer)=0) then ((State Sf automaton_buffer,(tsynbNull ds\<guillemotright>)))
-       else  (State Sf automaton_buffer, ((tsynbNull ds\<guillemotright>))))"  |
+lift_definition SenderAutomaton :: "(SenderState, abpMessage tsyn) dAutomaton" is "(senderTransition, State Sf [], (tsynbNull (\<C> ''ds'')), {\<C> ''i'', \<C> ''as''}, {\<C> ''ds''})"
+  by simp
 
-    "senderTransitionH (State St automaton_buffer, (Msg (A a), Msg (B b))) = 
-       (if((size automaton_buffer)>0 \<and> b=False) then ((State St ((prepend automaton_buffer)a),(createDsOutput (Pair (last automaton_buffer) True ))))
-       else if((size automaton_buffer)=1 \<and> b=True) then ((State Sf ((prepend (butlast automaton_buffer))a),(createDsOutput (Pair a False ))))
-       else if((size automaton_buffer)=0) then ((State St ((prepend automaton_buffer)a),(createDsOutput (Pair a True ))))
-       else if((size automaton_buffer)>1 \<and> b=True) then ((State Sf ((prepend (butlast automaton_buffer))a),(createDsOutput (Pair (last (butlast automaton_buffer)) False ))))
-       else  (State St automaton_buffer, ((tsynbNull ds\<guillemotright>))))"  |
-
-    "senderTransitionH (State St automaton_buffer, (null, Msg (B b))) = 
-       (if((size automaton_buffer)=0) then ((State St automaton_buffer,(tsynbNull ds\<guillemotright>)))
-       else if((size automaton_buffer)>1 \<and> b=True) then ((State Sf ((butlast automaton_buffer)),(createDsOutput (Pair (last (butlast automaton_buffer)) False ))))
-       else if((size automaton_buffer)=1 \<and> b=True) then ((State Sf ((butlast automaton_buffer)),(tsynbNull ds\<guillemotright>)))
-       else if((size automaton_buffer)>0 \<and> b=False) then ((State St automaton_buffer,(createDsOutput (Pair (last automaton_buffer) True ))))
-       else  (State St automaton_buffer, ((tsynbNull ds\<guillemotright>))))"  |
-
-    "senderTransitionH (State St automaton_buffer, (Msg (A a), null)) = 
-       (if((size automaton_buffer)>0) then ((State St ((prepend automaton_buffer)a),(createDsOutput (Pair (last automaton_buffer) True ))))
-       else if((size automaton_buffer)=0) then ((State St ((prepend automaton_buffer)a),(createDsOutput (Pair a True ))))
-       else  (State St automaton_buffer, ((tsynbNull ds\<guillemotright>))))"  |
-
-    "senderTransitionH (State St automaton_buffer, (null, null)) = 
-       (if((size automaton_buffer)>0) then ((State St automaton_buffer,(createDsOutput (Pair (last automaton_buffer) True ))))
-       else if((size automaton_buffer)=0) then ((State St automaton_buffer,(tsynbNull ds\<guillemotright>)))
-       else  (State St automaton_buffer, ((tsynbNull ds\<guillemotright>))))"  
-
-fun senderTransition :: "(SenderState \<times> (channel \<rightharpoonup> Sender tsyn)) \<Rightarrow> (SenderState \<times> Sender tsyn SB)" where
-"senderTransition (s,f) = (if dom(f) = {\<guillemotright>i,\<guillemotright>as} then senderTransitionH (s,(f\<rightharpoonup>\<guillemotright>i,f\<rightharpoonup>\<guillemotright>as)) else undefined)"
-
-lift_definition SenderAutomaton :: "(SenderState, Sender tsyn) automaton" is "(senderTransition, State Sf [], (tsynbNull ds\<guillemotright>), {c1,c2}, {c3})"
-sorry
-
-definition SenderSPF :: "Sender tsyn SPF" where
-"SenderSPF = H SenderAutomaton"
+definition SenderSPF :: "abpMessage tsyn SPF" where
+"SenderSPF = da_H SenderAutomaton"
 
 end
